@prefix : <http://crossings.github.io/term/> .
@prefix dc: <http://purl.org/dc/terms/> .
@prefix crm: <http://erlangen-crm.org/current/> .
@prefix owl: <http://www.w3.org/2002/07/owl#> .
@prefix rdf: <http://www.w3.org/1999/02/22-rdf-syntax-ns#> .
@prefix xml: <http://www.w3.org/XML/1998/namespace> .
@prefix xsd: <http://www.w3.org/2001/XMLSchema#> .
@prefix rdfs: <http://www.w3.org/2000/01/rdf-schema#> .
@prefix cucoo: <http://www.semanticweb.org/paulagranadosgarcia/CuCoO/> .
@base <http://crossings.github.io/CuCoO/core> .

<http://crossings.github.io/CuCoO/core> rdf:type owl:Ontology ;
                                         dc:creator <http://orcid.org/0000-0001-8029-7286> ,
                                                    <http://orcid.org/0000-0002-9272-908X> ,
                                                    <http://orcid.org/0000-0003-2014-0855> ;
                                         dc:description "This ontology defines the main concepts related to cross-cultural contact in history."@en ;
                                         dc:license <http://creativecommons.org/licenses/by-sa/4.0/> ;
                                         dc:title "CuCoO: The Cultural Contact Ontology - Core"@en ;
                                         rdfs:comment "Built upon on CuCoO - the Cultural Contact Ontology, by Paula Granados Garcia, CC BY-SA 2.0."@en .

#################################################################
#    Annotation properties
#################################################################

###  http://purl.org/dc/terms/creator
dc:creator rdf:type owl:AnnotationProperty .


###  http://purl.org/dc/terms/description
dc:description rdf:type owl:AnnotationProperty .


###  http://purl.org/dc/terms/license
dc:license rdf:type owl:AnnotationProperty .


###  http://purl.org/dc/terms/title
dc:title rdf:type owl:AnnotationProperty .


#################################################################
#    Object Properties
#################################################################

###  http://www.semanticweb.org/paulagranadosgarcia/CuCoO/hasAspect
cucoo:hasAspect rdf:type owl:ObjectProperty ;
                rdfs:domain cucoo:CulturalAgent ;
                rdfs:range cucoo:CulturalContactAspects ;
                rdfs:comment "Relates a CulutralContactAgent (e.g. coin) with the CulutralContactAspect featured (e.g. Linguistic)." .


###  http://www.semanticweb.org/paulagranadosgarcia/CuCoO/hasContext
cucoo:hasContext rdf:type owl:ObjectProperty ;
                 rdfs:domain cucoo:CulturalAgent ;
                 rdfs:range cucoo:CulturalContactContext ;
                 rdfs:comment "Relates a CulturalConceptAgent (e.g. sculpture) with the CulturalContact Context whose finding is related to (e.g. conquest)." .


###  http://www.semanticweb.org/paulagranadosgarcia/CuCoO/hasCulturalAssociation
cucoo:hasCulturalAssociation rdf:type owl:ObjectProperty ;
                             rdfs:domain cucoo:CulturalAgent ;
                             rdfs:comment "Relates an object with a culutral Association (e.g. Sculpture has culutral association clothing)." .


###  http://www.semanticweb.org/paulagranadosgarcia/CuCoO/hasCulturalContact
cucoo:hasCulturalContact rdf:type owl:ObjectProperty ;
                         rdfs:domain cucoo:CulturalContact ;
                         rdfs:range cucoo:CulturalAgent .


###  http://www.semanticweb.org/paulagranadosgarcia/CuCoO/hasCulturalIdentity
cucoo:hasCulturalIdentity rdf:type owl:ObjectProperty ;
                          rdfs:domain cucoo:CulturalAgent ;
                          rdfs:range cucoo:CulturalIdentity ;
                          rdfs:comment "Relates a Cultural Trait with the cultural Identitiy it is associated with (e.g. Toga has cultural identitity Roman)." .


###  http://www.semanticweb.org/paulagranadosgarcia/CuCoO/hasCulturalTrait
cucoo:hasCulturalTrait rdf:type owl:ObjectProperty ;
                       rdfs:domain cucoo:CulturalAgent ;
                       rdfs:range cucoo:CulturalContactTrait .


###  http://www.semanticweb.org/paulagranadosgarcia/CuCoO/isAssociatedWith
cucoo:isAssociatedWith rdf:type owl:ObjectProperty ;
                       rdfs:domain cucoo:CulturalAgent ,
                                   cucoo:CulturalContactTrait ;
                       rdfs:range cucoo:CulturalIdentity ;
                       rdfs:comment "Associates a CulturalContactTrait with a cultural identity." .


#################################################################
#    Classes
#################################################################

###  http://www.semanticweb.org/paulagranadosgarcia/CuCoO/Conquest
cucoo:Conquest rdf:type owl:Class ;
               rdfs:subClassOf cucoo:CulturalContactContext ;
               rdfs:comment "The cultural contact situation happens during a process of colonial conquest (e.g. Roman colonisation of the Iberian Penisula)." ;
               rdfs:label "conquest"@en .


###  http://www.semanticweb.org/paulagranadosgarcia/CuCoO/CulturalAgent
cucoo:CulturalAgent rdf:type owl:Class ;
                    rdfs:comment "Refers to things and people that embody and enact cultural meaning." ;
                    rdfs:label "bearer of cultural meaning"@en .


###  http://www.semanticweb.org/paulagranadosgarcia/CuCoO/CulturalContact
cucoo:CulturalContact rdf:type owl:Class ;
                      dc:description "Refers to the phenomenon of interaction amongst at least two communities with different cultural and ethnical backgrounds."@en ;
                      rdfs:label "cultural contact"@en .


###  http://www.semanticweb.org/paulagranadosgarcia/CuCoO/CulturalContactAspects
cucoo:CulturalContactAspects rdf:type owl:Class ;
                             rdfs:subClassOf cucoo:CulturalContactFeature ;
                             rdfs:comment "Character of the cultural contact situation (e.g. Economic, the evidence can prove the establishment of some economic relationship amongst the different comunities involved in the situation of cultural contact)." ;
                             rdfs:label "cultural contact aspect"@en .


###  http://www.semanticweb.org/paulagranadosgarcia/CuCoO/CulturalContactContext
cucoo:CulturalContactContext rdf:type owl:Class ;
                             rdfs:subClassOf cucoo:CulturalContactFeature ;
                             rdfs:comment "Refers to the context in which the situation of cultural contact takes place (e.g. in a context of trade, the main objective behind the cultural contact is economic profit)." ;
                             rdfs:label "cultural contact context"@en .


###  http://www.semanticweb.org/paulagranadosgarcia/CuCoO/CulturalContactFeature
cucoo:CulturalContactFeature rdf:type owl:Class ;
                             rdfs:comment "Refers to any cultural contact feature that can be identified in the entities. For example, cultural contact traits or cultural contact aspects." ;
                             rdfs:label "cultural contact feature"@en .


###  http://www.semanticweb.org/paulagranadosgarcia/CuCoO/CulturalContactTrait
cucoo:CulturalContactTrait rdf:type owl:Class ;
                           rdfs:subClassOf cucoo:CulturalContactFeature ;
                           rdfs:comment "Characteristic of human action accquired and transmited by any kind of communication in a situation of cultural contact." ;
                           rdfs:label "cultural contact trait"@en .


###  http://www.semanticweb.org/paulagranadosgarcia/CuCoO/CulturalIdentity
cucoo:CulturalIdentity rdf:type owl:Class ;
                       dc:description "Self-conscious association of a group or a person with a culturally constructed group identitiy that intersect with others in the identification of, and interaction, between groups. Refers to the elements that constitute a person's cultural identity."@en ;
                       rdfs:comment "Examples: being a Roman, a member of the Hakka people, a female or a hippie"@en ;
                       rdfs:label "cultural identity"@en .


###  http://www.semanticweb.org/paulagranadosgarcia/CuCoO/Iconographic
cucoo:Iconographic rdf:type owl:Class ;
                   rdfs:subClassOf cucoo:CulturalContactAspects ;
                   rdfs:comment "Iconographic influence amongst the different cultural groups can be demonstrated in  the evidence (e.g. spread of iconographic patterns)." ;
                   rdfs:label "iconographic aspect of cultural contact"@en .


###  http://www.semanticweb.org/paulagranadosgarcia/CuCoO/ImpermeableCulturalContact
cucoo:ImpermeableCulturalContact rdf:type owl:Class ;
                                 rdfs:subClassOf cucoo:CulturalContact ;
                                 owl:disjointWith cucoo:PermeableCulturalContact ;
                                 dc:description "Situation of cultural contact where there is no evidence for cultural influence."@en ;
                                 rdfs:comment "Example: the foundation of a colonia by the Romans did not cause the appearance of indigenous influences in material culture."@en ;
                                 rdfs:label "impermeable cultural contact"@en .


###  http://www.semanticweb.org/paulagranadosgarcia/CuCoO/Linguistic
cucoo:Linguistic rdf:type owl:Class ;
                 rdfs:subClassOf cucoo:CulturalContactAspects ;
                 rdfs:comment "Linguistic influence amongst the different cultural groups can be demonstrated in the evidence (e.g. bilingual inscriptions or use of foreign alphabets to record indigenous onomastica)." ;
                 rdfs:label "linguistic aspect of cultural contact"@en .


###  http://www.semanticweb.org/paulagranadosgarcia/CuCoO/PermeableCulturalContact
cucoo:PermeableCulturalContact rdf:type owl:Class ;
                               rdfs:subClassOf cucoo:CulturalContact ;
                               dc:description "Situation of cultural contact where there is evidence of cultural influence."@en ;
                               rdfs:comment "Example: the Roman conquest of the Iberian Peninsula caused appearance of Roman influences in the local material culture." ;
                               rdfs:label "permeable cultural contact"@en .


###  http://www.semanticweb.org/paulagranadosgarcia/CuCoO/Trade
cucoo:Trade rdf:type owl:Class ;
            rdfs:subClassOf cucoo:CulturalContactContext ;
            rdfs:comment "The cultural contact situation happens during a process of trade (e.g. Phoenician and Greek settlements in the peninsula)." ;
            rdfs:label "trade"@en .


###  Generated by the OWL API (version 4.5.9.2019-02-01T07:24:44Z) https://github.com/owlcs/owlapi
